fix Karatsuba's mult

code/experimental/rsa/Hacl.Impl.Comparison.fst
@@ -32,5 +32,32 @@ val bn_is_less:
     b:lbignum len -> Stack bool
     (requires (fun h -> live h a /\ live h b /\ disjoint a b))
     (ensures (fun h0 _ h1 -> preserves_live h0 h1 /\ h0 == h1))
-[@ "substitute"]    
+   
 let bn_is_less #len clen a b = bn_is_less_ #len clen a b clen
+
+val bn_is_less_ds_:
+    #a0Len:size_nat -> #a1Len:size_nat ->
+    aa0Len:size_t{v aa0Len == a0Len} -> a0:lbignum a0Len ->
+    aa1Len:size_t{v aa1Len == a1Len /\ a1Len <= a0Len} -> a1:lbignum a1Len ->
+    i:size_t{v i <= a0Len} -> Stack bool
+    (requires (fun h -> live h a0 /\ live h a1))
+    (ensures (fun h0 _ h1 -> preserves_live h0 h1 /\ h0 == h1))
+
+let rec bn_is_less_ds_ #a0Len #a1Len aa0Len a0 aa1Len a1 i =
+    if (i >. size 0) then
+        let i = size_decr i in
+        let t1 = a0.(i) in
+        let t2 = if (i <. aa1Len) then a1.(i) else u64 0 in
+        (if not (eq_u64 t1 t2) then
+            if lt_u64 t1 t2 then true else false
+        else bn_is_less_ds_ aa0Len a0 aa1Len a1 i)
+    else false
+
+val bn_is_less_ds:
+    #a0Len:size_nat -> #a1Len:size_nat ->
+    aa0Len:size_t{v aa0Len == a0Len} -> a0:lbignum a0Len ->
+    aa1Len:size_t{v aa1Len == a1Len /\ a1Len <= a0Len} -> a1:lbignum a1Len -> Stack bool
+    (requires (fun h -> live h a0 /\ live h a1))
+    (ensures (fun h0 _ h1 -> preserves_live h0 h1 /\ h0 == h1))
+
+let bn_is_less_ds #a0Len #a1len aa0Len a0 aa1Len a1 = bn_is_less_ds_ aa0Len a0 aa1Len a1 aa0Len
