code/experimental/rsa/Hacl.Impl.Exponentiation.fst
@@ -15,67 +15,69 @@ module Buffer = Spec.Lib.IntBuf
 
 val mul_mod_mont:
     #rLen:size_nat ->
-    iLen:size_t{8 * v iLen < max_size_t /\ rLen <= v iLen} ->
+    pow2_i:size_t{rLen + rLen + 4 * v pow2_i < max_size_t /\ rLen < v pow2_i} -> iLen:size_t ->
     exp_r:size_t{0 < v exp_r /\ rLen = v exp_r / 64 + 1} ->
     rrLen:size_t{v rrLen == rLen /\ 0 < rLen /\ 6 * rLen < max_size_t} ->
     st_mont:lbignum (3 * rLen) ->
-    st_kara:lbignum (8 * v iLen) ->
-    aM:lbignum rLen -> bM:lbignum rLen ->
-    resM:lbignum rLen -> Stack unit
+    st_kara:lbignum (2 * rLen + 4 * v pow2_i) ->
+    aM:lbignum rLen -> bM:lbignum rLen -> resM:lbignum rLen -> Stack unit
     (requires (fun h -> live h st_mont /\ live h aM /\ live h bM /\ live h resM /\ live h st_kara))
     (ensures (fun h0 _ h1 -> preserves_live h0 h1))
-[@ "substitute"]
-let mul_mod_mont #rLen iLen exp_r rrLen st_mont st_kara aM bM resM =
-    let stLen = mul #SIZE (size 8) iLen in
+
+let mul_mod_mont #rLen pow2_i iLen exp_r rrLen st_mont st_kara aM bM resM =
     let cLen = add #SIZE rrLen rrLen in
+    let stKLen = mul #SIZE (size 4) pow2_i in
+    let stLen = add #SIZE cLen stKLen in
+    
     let c = Buffer.sub #uint64 #(v stLen) #(v cLen) st_kara (size 0) cLen in
+    let st_k = Buffer.sub #uint64 #(v stLen) #(v stKLen) st_kara cLen stKLen in
     let st = Buffer.sub #uint64 #(v stLen) #(3 * rLen) st_kara cLen (mul #SIZE (size 3) rrLen) in
     //fill cLen c (u64 0);
     //bn_mul rrLen aM rrLen bM c;
-    karatsuba iLen rrLen aM bM st_kara; // c = a * b
+    karatsuba pow2_i iLen rrLen aM bM st_k c; // c = a * b
     mont_reduction exp_r rrLen st_mont st cLen c resM // resM = c % n
    
 val mod_exp_:
     #rLen:size_nat -> #bLen:size_nat ->
-    iLen:size_t{8 * v iLen < max_size_t /\ rLen <= v iLen} ->
+    pow2_i:size_t{rLen + rLen + 4 * v pow2_i < max_size_t /\ rLen < v pow2_i} -> iLen:size_t ->
     exp_r:size_t{0 < v exp_r /\ rLen = v exp_r / 64 + 1} ->
     rrLen:size_t{v rrLen == rLen /\ 0 < rLen /\ 6 * rLen < max_size_t} ->
     st_mont:lbignum (3 * rLen) ->
     st_exp:lbignum (2 * rLen) ->
-    st_kara:lbignum (8 * v iLen) ->
+    st_kara:lbignum (2 * rLen + 4 * v pow2_i) ->
     bBits:size_t{0 < v bBits} ->
     bbLen:size_t{v bbLen == bLen /\ bLen = v (bits_to_bn bBits) /\ v bBits / 64 <= bLen} ->
     b:lbignum bLen ->
     count:size_t{v count <= v bBits} -> Stack unit
-    (requires (fun h -> live h st_mont /\ live h st_exp /\ live h b))
-    (ensures  (fun h0 _ h1 -> preserves_live h0 h1 /\ modifies1 st_exp h0 h1))
+    (requires (fun h -> live h st_mont /\ live h st_exp /\ live h b /\ live h st_kara))
+    (ensures  (fun h0 _ h1 -> preserves_live h0 h1))
 
 #reset-options "--z3rlimit 50 --max_fuel 0 --max_ifuel 0 "
 
-let rec mod_exp_ #rLen #bLen iLen exp_r rrLen st_mont st_exp st_kara bBits bbLen b count =
+let rec mod_exp_ #rLen #bLen pow2_i iLen exp_r rrLen st_mont st_exp st_kara bBits bbLen b count =
     let aM = Buffer.sub #uint64 #(rLen + rLen) #rLen st_exp (size 0) rrLen in
     let accM = Buffer.sub #uint64 #(rLen + rLen) #rLen st_exp rrLen rrLen in
     
     if (count <. bBits) then begin
         (if (bn_is_bit_set bbLen b count) then begin
-            mul_mod_mont iLen exp_r rrLen st_mont st_kara aM accM accM end); //acc = (acc * a) % n
-        mul_mod_mont iLen exp_r rrLen st_mont st_kara aM aM aM; //a = (a * a) % n
-	mod_exp_ iLen exp_r rrLen st_mont st_exp st_kara bBits bbLen b (size_incr count)
+            mul_mod_mont pow2_i iLen exp_r rrLen st_mont st_kara aM accM accM end); //acc = (acc * a) % n
+        mul_mod_mont pow2_i iLen exp_r rrLen st_mont st_kara aM aM aM; //a = (a * a) % n
+	mod_exp_ pow2_i iLen exp_r rrLen st_mont st_exp st_kara bBits bbLen b (size_incr count)
     end
 
 val mod_exp_mont:
     #rLen:size_nat -> #stLen:size_nat ->
-    iLen:size_t{8 * v iLen < max_size_t /\ rLen <= v iLen} ->
+    pow2_i:size_t{rLen + rLen + 4 * v pow2_i < max_size_t /\ rLen < v pow2_i} -> iLen:size_t ->
     bBits:size_t{0 < v bBits} -> b:lbignum (v (bits_to_bn bBits)) ->
     exp_r:size_t{0 < v exp_r /\ rLen = v exp_r / 64 + 1} ->
     rrLen:size_t{v rrLen == rLen /\ 0 < rLen /\ 9 * rLen < max_size_t} ->
-    sstLen:size_t{v sstLen == stLen /\ stLen = 9 * rLen + 8 * v iLen} -> st:lbignum stLen -> Stack unit
+    sstLen:size_t{v sstLen == stLen} -> st:lbignum stLen -> Stack unit
     (requires (fun h -> live h b /\ live h st /\ disjoint st b))
     (ensures (fun h0 _ h1 -> preserves_live h0 h1 /\ modifies1 st h0 h1))
 
 #reset-options "--z3rlimit 150 --max_fuel 0 --max_ifuel 0"
-[@ "substitute"]
-let mod_exp_mont #rLen #stLen iLen bBits b exp_r rrLen sstLen st =
+
+let mod_exp_mont #rLen #stLen pow2_i iLen bBits b exp_r rrLen sstLen st =
     let bLen = bits_to_bn bBits in
     assert (v bBits / 64 <= v bLen);
     
@@ -92,23 +94,25 @@ let mod_exp_mont #rLen #stLen iLen bBits b exp_r rrLen sstLen st =
     
     let st_mont = Buffer.sub #uint64 #stLen #(3 * rLen) st (size 0) (mul #SIZE (size 3) rrLen) in
     let st_exp = Buffer.sub #uint64 #stLen #(2 * rLen) st (mul #SIZE (size 6) rrLen) (mul #SIZE (size 2) rrLen) in
-    let st_kara = Buffer.sub #uint64 #stLen #(8 * v iLen) st (mul #SIZE (size 9) rrLen) (mul #SIZE (size 8) iLen) in
+    let stKLen = add #SIZE (mul #SIZE (size 2) rrLen) (mul #SIZE (size 4) pow2_i) in
+    let st_kara = Buffer.sub #uint64 #stLen #(v stKLen) st (mul #SIZE (size 9) rrLen) stKLen in
     let st_t = Buffer.sub #uint64 #stLen #(5 * rLen) st (mul #SIZE (size 9) rrLen) (mul #SIZE (size 5) rrLen) in
     let st_f = Buffer.sub #uint64 #stLen #(3 * rLen) st (mul #SIZE (size 9) rrLen) (mul #SIZE (size 3) rrLen) in
     to_mont exp_r rrLen st_mont st_t r2 a1 aM;
     to_mont exp_r rrLen st_mont st_t r2 acc accM;
 
-    mod_exp_ iLen exp_r rrLen st_mont st_exp st_kara bBits bLen b (size 0);
+    mod_exp_ pow2_i iLen exp_r rrLen st_mont st_exp st_kara bBits bLen b (size 0);
     from_mont exp_r rrLen st_mont st_f accM res1
     
 // res = a ^^ b mod n
 val mod_exp:
     #nLen:size_nat ->
-    iLen:size_t{8 * v iLen < max_size_t} ->
+    pow2_i:size_t -> iLen:size_t ->
     modBits:size_t{0 < v modBits /\ 2 * v modBits + 4 < max_size_t} ->
-    nnLen:size_t{v nnLen == nLen /\ 0 < nLen /\ nLen = v (bits_to_bn modBits) /\ 
-		 9 * v (bits_to_bn (add #SIZE modBits (size 2))) < max_size_t /\
-		 v (bits_to_bn (add #SIZE modBits (size 2))) <= v iLen} ->
+    nnLen:size_t{let rLen = v (bits_to_bn (add #SIZE modBits (size 2))) in
+                 v nnLen == nLen /\ 0 < nLen /\ nLen = v (bits_to_bn modBits) /\
+		 9 * rLen < max_size_t /\ 2 * rLen + 4 * v pow2_i < max_size_t /\
+		 rLen < v pow2_i} ->
     n:lbignum nLen -> a:lbignum nLen ->
     bBits:size_t{0 < v bBits} -> b:lbignum (v (bits_to_bn bBits)) ->
     res:lbignum nLen -> Stack unit
@@ -117,7 +121,7 @@ val mod_exp:
     
 #reset-options "--lax"
 
-let mod_exp #nLen iLen modBits nnLen n a bBits b res =
+let mod_exp #nLen pow2_i iLen modBits nnLen n a bBits b res =
     let exp_r = add #SIZE modBits (size 2) in
     let rBits = add #SIZE modBits (size 3) in
     let rLen = bits_to_bn rBits in
@@ -128,7 +132,7 @@ let mod_exp #nLen iLen modBits nnLen n a bBits b res =
     assert (v exp_r / 64 < v rLen);
     assert (v modBits / 64 < v rLen);
 
-    let stLenKara = mul #SIZE (size 8) iLen in
+    let stLenKara = add #SIZE (mul #SIZE (size 2) rLen) (mul #SIZE (size 4) pow2_i) in
     let stLen' = mul #SIZE (size 9) rLen in
     let stLen = add #SIZE stLenKara stLen' in
     let stMLen = mul #SIZE (size 3) rLen in
@@ -159,7 +163,7 @@ let mod_exp #nLen iLen modBits nnLen n a bBits b res =
       bn_set_bit rLen r exp_r; // r = pow2 (2 + modBits)
       bn_pow2_mod_n modBits rLen n1 exp2 r2; // r2 = r * r % n
       mont_inverse rLen n1 exp_r nInv; // n * nInv = 1 (mod r)
-      mod_exp_mont #(v rLen) #(v stLen) iLen bBits b exp_r rLen stLen st;
+      mod_exp_mont #(v rLen) #(v stLen) pow2_i iLen bBits b exp_r rLen stLen st;
       
       copy nnLen res1_ res
     )
